
\documentclass[12pt]{article}
\usepackage{amsmath}
\DeclareMathOperator*{\argmin}{arg\,min} % thin space, limits underneath in displays
\DeclareMathOperator*{\argmax}{arg\,max} % thin space, limits underneath in displays
\newtheorem{thm}{Theorem}
\usepackage{amssymb}
\usepackage{amsfonts}
\usepackage{mathrsfs}
\usepackage{bm}
\usepackage{indentfirst}
\setlength{\parindent}{0em}
\usepackage[margin=1in]{geometry}
\usepackage{graphicx}
\usepackage{setspace}
\doublespacing
\usepackage[flushleft]{threeparttable}
\usepackage{booktabs,caption}
\usepackage{float}
\usepackage{graphicx}
\usepackage[sort,comma]{natbib}
\usepackage[hidelinks]{hyperref}

\usepackage{import}
\usepackage{xifthen}
\usepackage{pdfpages}
\usepackage{transparent}

\newcommand{\incfig}[1]{%
\def\svgwidth{\columnwidth}
\import{./figures/}{#1.pdf_tex}
}




\title{}
\author{}
\date{}


\begin{document}
\maketitle


\section{$ \int_{}^{} xe^{x}dx $}


To solve this, we need this
\begin{equation*}
\int_{}^{} udv = uv - \int_{}^{} v du
\end{equation*}
Let $ u = x $, then $ dv = e^{x}dx $. We can also know $ du = dx $.

What is $ v $?
\begin{align*}
v &= \int_{}^{} dv = \int_{}^{} e^{x}dx\\
&= e^{x}
\end{align*}

Now we can solve this question:
\begin{align*}
\int_{}^{} xe^{x}dx &= \int_{}^{} u dv = uv - \int_{}^{} vdu\\
&= xe^{x} - \int_{}^{} e^{x}dx\\
&= xe^{x} - e^{x} + c
\end{align*}




{\textbf {Solve the mean of the exponential distribution}}\\
Give the density of the exponential distribution:
\begin{equation*}
f(x;\lambda) = \lambda e^{ - \lambda x}, \lambda \in \mathbb{R}_{+}, x \in \mathbb{R}
_{+}
\end{equation*}
\begin{align*}
E(x)&= \int_{0}^{\infty } x \lambda e^{ - \lambda x}dx\\
&= \lambda \int_{0}^{\infty } x e^{ - \lambda x}dx\\
u = x &, dv =  e^{ - \lambda x}dx\\
v&= \int_{}^{} dv = \int_{}^{}  e^{ - \lambda x}dx =  - \frac{1}{\lambda}e^{ - \lambda
x}\\
E(x) = \lambda \int_{0}^{\infty } xe^{ - \lambda x}dx
&= \lambda \left[ uv \Bigg|^{\infty }_{0} - \int_{0}^{\infty }vdu  \right] \\
&= \lambda \left[  - \frac{x}{\lambda}e^{ - \lambda x} \Bigg|^{\infty }_{0}
 - \int_{0}^{\infty } - \frac{1}{\lambda}e^{ - \lambda x} dx \right] \\
&= \lambda \left[ 0 + \frac{1}{\lambda} 
\left(  - \frac{1}{\lambda} e^{ - \lambda x} \right) \Bigg|^{\infty }_{0} \right] \\
&= 0 - ( - \frac{1}{\lambda})\\
E(x)&= \frac{1}{\lambda}
\end{align*}





\section{Taylor Exansion}
\begin{align*}
f(x)&= \sum\limits_{n = 0} ^\infty \frac{f^{(n)}(a)(x - a)^{n}}{n!}\\
&= \frac{f(a)\cdot 1}{1} + f'(a)(x - a) + \frac{1}{2}f''(a)(x - a)^{2} + ...
\end{align*}
where
\begin{equation*}
f^{(0)}(a) = f(a), \quad 0! = 1
\end{equation*}







\bibliographystyle{plainnat}
\bibliography{my_bib}

\end{document}

